\documentclass{article}
\usepackage{epsfig}
\usepackage{amssymb,amsmath}
\pagestyle{empty}
\begin{document}
${\bf s}(t) \in \mathbb{R}^n $
\pagebreak

$ t $
\pagebreak

${\bf s}^*(t) $
\pagebreak

$ e(t) = {\bf s}^*(t) - {\bf s}(t) $
\pagebreak

$ \frac{\delta {\bf s}(t)}{\delta {\bf q}(t)}$
\pagebreak

$ {\bf s}^*(t) $
\pagebreak

$ [ 0 1 0] $
\pagebreak

$ {\bf s}^*(t) - {\bf s}(t)$
\pagebreak

$ J(t) = \frac{\delta{\bf s}^*(t)}{\delta {\bf q}(t)}$
\pagebreak

$ {\bf s}(t)$
\pagebreak

${\bf x}_{k \mid k} $
\pagebreak

${\bf x}_{k \mid k} = {\bf x}_{k \mid k-1} + {\bf W}_k \left[ {\bf z}_k - {\bf H x}_{k \mid k-1} \right]$
\pagebreak

${\bf x}_{k \mid k-1} $
\pagebreak

$ {{\bf x}}_{k|k-1} = {\bf A}_{k-1} {\bf x}_{k-1\mid k-1}$
\pagebreak

${\bf P}_{k \mid k-1} $
\pagebreak

$ {\bf A}_{k-1} {\bf P}_{k-1 \mid k-1} {\bf A}^T_{k-1} + {\bf Q}_k$
\pagebreak

${\bf P}_{k \mid k}$
\pagebreak

${\bf P}_{k \mid k} = \left({\bf I - W}_k {\bf H} \right) {\bf P}_{k \mid k-1}$
\pagebreak

${\bf W}_k$
\pagebreak

$ {\bf W}_k = {\bf P}_{k \mid k-1} {\bf H}^T \left[ {\bf H P}_{k \mid k-1} {\bf H}^T + {\bf R}_k \right]^{-1}$
\pagebreak

$ \bf I$
\pagebreak

$ {\bf s} ={\bf e}({\bf q}) $
\pagebreak

${\bf s} $
\pagebreak

${\bf q}$
\pagebreak

$ {\bf e} = - \lambda \dot{\bf e} $
\pagebreak

$ {\bf J} = \frac{\delta f}{\delta {\bf q}} $
\pagebreak

$ \dot{\bf q} = -\lambda {\bf J}^{\#} \dot{\bf e}$
\pagebreak

$ \dot{\bf e} = {\bf s}^{des} - {\bf s}^* $
\pagebreak

$ {\bf s}^{des}$
\pagebreak

$ {\bf s}^* $
\pagebreak

\end{document}
